mem/Mem1.v
@@ -10,13 +10,11 @@ Require Import HoareDef.
 Require Import TODOYJ.
 Require Import Logic.
 
-Generalizable Variables E R A B C X Y Σ.
-
 Set Implicit Arguments.
 
 
 
-Let _memRA: URA.t := (block ==> Z ==> (Excl.t val))%ra.
+Let _memRA: URA.t := (mblock ==> Z ==> (Excl.t val))%ra.
 Compute (URA.car (t:=_memRA)).
 Instance memRA: URA.t := Auth.t _memRA.
 Compute (URA.car).
@@ -24,7 +22,7 @@ Compute (URA.car).
 Section PROOF.
   Context `{@GRA.inG memRA Σ}.
 
-  Definition _points_to (loc: block * Z) (vs: list val): _memRA :=
+  Definition _points_to (loc: mblock * Z) (vs: list val): _memRA :=
     let (b, ofs) := loc in
     (fun _b _ofs => if (dec _b b) && ((ofs <=? _ofs) && (_ofs <? (ofs + Z.of_nat (List.length vs))))%Z
                     then (List.nth_error vs (Z.to_nat (_ofs - ofs))) else ε)
@@ -39,7 +37,7 @@ Section PROOF.
   .
   Proof. refl. Qed.
 
-  Definition points_to (loc: block * Z) (vs: list val): memRA := Auth.white (_points_to loc vs).
+  Definition points_to (loc: mblock * Z) (vs: list val): memRA := Auth.white (_points_to loc vs).
 
   Lemma points_to_split
         blk ofs hd tl
@@ -48,31 +46,31 @@ Section PROOF.
   .
   Proof.
     ss. unfold points_to. unfold Auth.white. repeat (rewrite URA.unfold_add; ss).
-    f_equal.
-    repeat (apply func_ext; i).
+    f_equal. unfold URA.car. ss.
+    repeat (apply Axioms.func_ext; i).
     des_ifs; bsimpl; des; des_sumbool; subst; ss;
-      try rewrite Z.leb_gt in *; try rewrite Z.leb_le in *; try rewrite Z.ltb_ge in *; try rewrite Z.ltb_lt in *; try lia.
-    - clear_tac. subst. rewrite Zpos_P_of_succ_nat in *. rewrite <- Zlength_correct in *.
+      try erewrite Z.leb_gt in *; try erewrite Z.leb_le in *; try erewrite Z.ltb_ge in *; try erewrite Z.ltb_lt in *; try lia.
+    - clear_tac. subst. try erewrite Zpos_P_of_succ_nat in *. try erewrite <- Zlength_correct in *.
       assert(x0 = ofs). { lia. } subst.
-      rewrite Z.sub_diag in *. ss.
-    - clear_tac. rewrite Zpos_P_of_succ_nat in *. rewrite <- Zlength_correct in *.
+      erewrite Z.sub_diag in *. ss.
+    - clear_tac. try erewrite Zpos_P_of_succ_nat in *. erewrite <- Zlength_correct in *.
       destruct (Z.to_nat (x0 - ofs)) eqn:T; ss.
       { exfalso. lia. }
-      rewrite Z.sub_add_distr in *. rewrite Z2Nat.inj_sub in Heq1; ss. rewrite T in *. ss. rewrite Nat.sub_0_r in *. ss.
-    - clear_tac. rewrite Zpos_P_of_succ_nat in *. rewrite <- Zlength_correct in *.
+      erewrite Z.sub_add_distr in *. rewrite Z2Nat.inj_sub in Heq1; ss. erewrite T in *. ss. erewrite Nat.sub_0_r in *. ss.
+    - clear_tac. try erewrite Zpos_P_of_succ_nat in *. erewrite <- Zlength_correct in *.
       destruct (Z.to_nat (x0 - ofs)) eqn:T; ss.
       { exfalso. lia. }
-      rewrite Z.sub_add_distr in *. rewrite Z2Nat.inj_sub in Heq1; ss. rewrite T in *. ss. rewrite Nat.sub_0_r in *. ss.
-    - clear_tac. rewrite Zpos_P_of_succ_nat in *. rewrite <- Zlength_correct in *.
+      erewrite Z.sub_add_distr in *. rewrite Z2Nat.inj_sub in Heq1; ss. erewrite T in *. ss. erewrite Nat.sub_0_r in *. ss.
+    - clear_tac. try erewrite Zpos_P_of_succ_nat in *. try erewrite <- Zlength_correct in *.
       assert(x0 = ofs). { lia. } subst.
-      rewrite Z.sub_diag in *. ss.
-    - clear_tac. rewrite Zpos_P_of_succ_nat in *. rewrite <- Zlength_correct in *.
+      erewrite Z.sub_diag in *. ss.
+    - clear_tac. try erewrite Zpos_P_of_succ_nat in *. erewrite <- Zlength_correct in *.
       destruct (Z.to_nat (x0 - ofs)) eqn:T; ss.
       { exfalso. lia. }
-      rewrite Z.sub_add_distr in *. rewrite Z2Nat.inj_sub in Heq1; ss. rewrite T in *. ss. rewrite Nat.sub_0_r in *. ss.
-    - clear_tac. rewrite Zpos_P_of_succ_nat in *. rewrite <- Zlength_correct in *.
+      erewrite Z.sub_add_distr in *. rewrite Z2Nat.inj_sub in Heq1; ss. erewrite T in *. ss. erewrite Nat.sub_0_r in *. ss.
+    - clear_tac. try erewrite Zpos_P_of_succ_nat in *. try erewrite <- Zlength_correct in *.
       assert(x0 = ofs). { lia. } subst.
-      rewrite Z.sub_diag in *. ss.
+      erewrite Z.sub_diag in *. ss.
   Qed.
 
 (* Lemma points_tos_points_to *)
@@ -112,46 +110,47 @@ Section PROOF.
   Let GURA: URA.t := GRA.to_URA Σ.
   Local Existing Instance GURA.
 
-  Definition alloc_spec: fspec :=
+  Let alloc_spec: fspec :=
     (mk_simple (fun sz => (
-                    (fun varg o => ⌜varg = [Vint (Z.of_nat sz)]↑ /\ o = ord_pure 0⌝),
-                    (fun vret => Exists b, ⌜vret = (Vptr b 0)↑⌝ **
-                                                             Own(GRA.embed ((b, 0%Z) |-> (List.repeat (Vint 0) sz))))
-    ))).
+                    (fun varg o => (⌜varg = [Vint (Z.of_nat sz)]↑ /\ o = ord_pure 0⌝: iProp)%I),
+                    (fun vret => (∃ b, ⌜vret = (Vptr b 0)↑⌝ **
+                                                         Own(GRA.embed ((b, 0%Z) |-> (List.repeat (Vint 0) sz))))%I
+    )))).
 
-  Definition free_spec: fspec :=
+  Let free_spec: fspec :=
     (mk_simple (fun '(b, ofs) => (
-                    (fun varg o => Exists v, ⌜varg = ([Vptr b ofs])↑⌝ **
-                                             Own(GRA.embed ((b, ofs) |-> [v])) **
-                                             ⌜o = ord_pure 0⌝),
-                    top2
+                    (fun varg o => (∃ v, ⌜varg = ([Vptr b ofs])↑⌝ **
+                                                               Own(GRA.embed ((b, ofs) |-> [v])) **
+                                                               ⌜o = ord_pure 0⌝: iProp)%I),
+                    (fun _ => (True: iProp)%I)
     ))).
 
-  Definition load_spec: fspec :=
+
+  Let load_spec: fspec :=
     (mk_simple (fun '(b, ofs, v) => (
-                    (fun varg o => ⌜varg = ([Vptr b ofs])↑⌝ **
-                                   Own(GRA.embed ((b, ofs) |-> [v])) **
-                                   ⌜o = ord_pure 0⌝),
+                    (fun varg o => (⌜varg = ([Vptr b ofs])↑⌝ **
+                                                          Own(GRA.embed ((b, ofs) |-> [v])) **
+                                                          ⌜o = ord_pure 0⌝: iProp)%I),
                     (fun vret => Own(GRA.embed ((b, ofs) |-> [v])) ** ⌜vret = v↑⌝)
     ))).
 
-  Definition store_spec: fspec :=
+  Let store_spec: fspec :=
     (mk_simple
        (fun '(b, ofs, v_new) => (
-            (fun varg o => Exists v_old,
-                           ⌜varg = ([Vptr b ofs ; v_new])↑⌝ ** Own(GRA.embed ((b, ofs) |-> [v_old])) ** ⌜o = ord_pure 0⌝),
+            (fun varg o => (∃ v_old,
+                               ⌜varg = ([Vptr b ofs ; v_new])↑⌝ ** Own(GRA.embed ((b, ofs) |-> [v_old])) ** ⌜o = ord_pure 0⌝: iProp)%I),
             (fun _ => Own(GRA.embed ((b, ofs) |-> [v_new])))
     ))).
 
-  Definition cmp_spec: fspec :=
+  Let cmp_spec: fspec :=
     (mk_simple
        (fun '(result, resource) => (
           (fun varg o =>
-          ((Exists b ofs v, ⌜varg = [Vptr b ofs; Vnullptr]↑⌝ ** ⌜resource = (GRA.embed ((b, ofs) |-> [v]))⌝ ** ⌜result = false⌝) ∨
-           (Exists b ofs v, ⌜varg = [Vnullptr; Vptr b ofs]↑⌝ ** ⌜resource = (GRA.embed ((b, ofs) |-> [v]))⌝ ** ⌜result = false⌝) ∨
-           (Exists b0 ofs0 v0 b1 ofs1 v1, ⌜varg = [Vptr b0 ofs0; Vptr b1 ofs1]↑⌝ **
+          ((∃ b ofs v, ⌜varg = [Vptr b ofs; Vnullptr]↑⌝ ** ⌜resource = (GRA.embed ((b, ofs) |-> [v]))⌝ ** ⌜result = false⌝) ∨
+           (∃ b ofs v, ⌜varg = [Vnullptr; Vptr b ofs]↑⌝ ** ⌜resource = (GRA.embed ((b, ofs) |-> [v]))⌝ ** ⌜result = false⌝) ∨
+           (∃ b0 ofs0 v0 b1 ofs1 v1, ⌜varg = [Vptr b0 ofs0; Vptr b1 ofs1]↑⌝ **
                      ⌜resource = (GRA.embed ((b0, ofs0) |-> [v0])) ⋅ (GRA.embed ((b1, ofs1) |-> [v1]))⌝ ** ⌜result = false⌝) ∨
-           (Exists b ofs v, ⌜varg = [Vptr b ofs; Vptr b  ofs]↑⌝ ** ⌜resource = (GRA.embed ((b, ofs) |-> [v]))⌝ ** ⌜result = true⌝) ∨
+           (∃ b ofs v, ⌜varg = [Vptr b ofs; Vptr b  ofs]↑⌝ ** ⌜resource = (GRA.embed ((b, ofs) |-> [v]))⌝ ** ⌜result = true⌝) ∨
            (⌜varg = [Vnullptr; Vnullptr]↑ /\ result = true⌝))
             ** Own(resource)
             ** ⌜o = ord_pure 0⌝
